theories/zoo/program_logic/bwp.v
@@ -901,7 +901,7 @@ Section zoo_G.
     iIntros "%He >#Hl H".
     iApply bwp_lift_base_step_nofork; first done. iIntros "%ns %nt %σ1 %κs Hinterp".
     iApply fupd_mask_intro; first set_solver. iIntros "Hclose".
-    iDestruct (state_interp_has_header_valid with "Hinterp Hl") as %Hheaders_lookup.
+    iDestruct (state_interp_headers_at_valid with "Hinterp Hl") as %Hheaders_lookup.
     iSplit; first eauto with zoo. iIntros "%κ %κs' %e_ %σ_ %es -> %Hstep _ !>".
     invert_base_step.
     iSteps.
